misc helper lemmas

semantics/prop/vyperEvalMiscScript.sml
@@ -1,7 +1,18 @@
 Theory vyperEvalMisc
 
 Ancestors
-  vyperInterpreter
+  vyperInterpreter vyperArray vyperTypeValue
+
+Libs
+  intLib wordsLib
+
+val within_int_bound_def = vyperTypeValueTheory.within_int_bound_def;
+val evaluate_binop_def = vyperInterpreterTheory.evaluate_binop_def;
+val bounded_int_op_def = vyperInterpreterTheory.bounded_int_op_def;
+val word_mod_def = wordsTheory.word_mod_def;
+val w2n_n2w = wordsTheory.w2n_n2w;
+val SIZES_CONV = wordsLib.SIZES_CONV;
+val ARITH_TAC = intLib.ARITH_TAC;
 
 Theorem eval_stmts_append:
   ∀cx ss1 ss2. eval_stmts cx (ss1 ++ ss2) = do eval_stmts cx ss1; eval_stmts cx ss2 od
@@ -53,4 +64,138 @@ Proof
                 SOME (ScopedVar n)
               else NONE) NONE` >>
   gvs[return_def, raise_def]
+QED
+
+(* ===== Binop Helper Lemmas ===== *)
+
+(* Unsigned modulo for uint256 % 3 *)
+Theorem evaluate_binop_mod_uint256_3:
+  ∀x.
+    within_int_bound (Unsigned 256) x ⇒
+    evaluate_binop Mod (IntV (Unsigned 256) x) (IntV (Unsigned 256) 3) =
+    INL (IntV (Unsigned 256) (x % 3))
+Proof
+  rpt strip_tac >> gvs[within_int_bound_def] >>
+  simp[evaluate_binop_def, bounded_int_op_def, within_int_bound_def] >>
+  (* Establish key equation: w2i (word_mod (i2w x) (i2w 3)) = x % 3 *)
+  sg `w2i (word_mod ((i2w x):bytes32) (i2w 3)) = x % 3` >- (
+    `x = &(Num x)` by gvs[integerTheory.INT_OF_NUM] >>
+    pop_assum SUBST_ALL_TAC >>
+    simp[integer_wordTheory.i2w_pos, word_mod_def, w2n_n2w] >>
+    CONV_TAC (DEPTH_CONV (TRY_CONV SIZES_CONV)) >> fs[] >>
+    simp[GSYM integer_wordTheory.i2w_pos] >>
+    irule integer_wordTheory.w2i_i2w_pos >>
+    CONV_TAC (RAND_CONV (TRY_CONV SIZES_CONV)) >>
+    `Num x MOD 3 < 3` by simp[] >> simp[]
+  ) >>
+  gvs[] >>
+  `0 ≤ x % 3 ∧ x % 3 < 3` by (
+    `(3:int) ≠ 0` by simp[] >>
+    drule integerTheory.INT_MOD_BOUNDS >>
+    disch_then (qspec_then `x` mp_tac) >> simp[]
+  ) >>
+  `x % 3 = 0 ∨ x % 3 = 1 ∨ x % 3 = 2` by ARITH_TAC >> gvs[]
+QED
+
+(* Bounds on x % 3 *)
+Theorem uint256_mod_3_bounds:
+  ∀x. 0 ≤ x ⇒ 0 ≤ x % 3 ∧ x % 3 < 3
+Proof
+  rpt strip_tac >>
+  `(3:int) ≠ 0` by simp[] >>
+  drule integerTheory.INT_MOD_BOUNDS >>
+  disch_then (qspec_then `x` mp_tac) >> simp[]
+QED
+
+(* Unsigned subtraction when y ≤ x *)
+Theorem evaluate_binop_sub_small_unsigned:
+  ∀x y.
+    within_int_bound (Unsigned 256) x ∧
+    within_int_bound (Unsigned 256) y ∧
+    y ≤ x ⇒
+    evaluate_binop Sub (IntV (Unsigned 256) x) (IntV (Unsigned 256) y) =
+    INL (IntV (Unsigned 256) (x − y))
+Proof
+  rpt strip_tac >>
+  simp[evaluate_binop_def, bounded_int_op_def] >>
+  gvs[within_int_bound_def] >>
+  `0 ≤ x - y` by ARITH_TAC >> simp[] >>
+  `Num (x - y) ≤ Num x` suffices_by simp[] >>
+  simp[integerTheory.INT_OF_NUM] >> ARITH_TAC
+QED
+
+(* Signed 128 addition when result is in bounds *)
+Theorem evaluate_binop_add_int128:
+  ∀a b.
+    within_int_bound (Signed 128) a ∧
+    within_int_bound (Signed 128) b ∧
+    within_int_bound (Signed 128) (a + b) ⇒
+    evaluate_binop Add (IntV (Signed 128) a) (IntV (Signed 128) b) =
+    INL (IntV (Signed 128) (a + b))
+Proof
+  rpt strip_tac >>
+  simp[evaluate_binop_def, bounded_int_op_def]
+QED
+
+(* ===== Array Init Properties ===== *)
+
+Definition arr_init_def:
+  arr_init = SArrayV (BaseTV (IntT 128)) 3
+    [(0, IntV (Signed 128) 10); (1, IntV (Signed 128) 11);
+     (2, IntV (Signed 128) 12)]
+End
+
+Theorem arr_init_make_array:
+  make_array_value (BaseTV (IntT 128)) (Fixed 3)
+    [IntV (Signed 128) 10; IntV (Signed 128) 11; IntV (Signed 128) 12] =
+  arr_init
+Proof
+  EVAL_TAC >> simp[arr_init_def]
+QED
+
+Theorem arr_init_index_0:
+  array_index arr_init 0 = SOME (IntV (Signed 128) 10)
+Proof
+  EVAL_TAC >> simp[arr_init_def]
+QED
+
+Theorem arr_init_index_1:
+  array_index arr_init 1 = SOME (IntV (Signed 128) 11)
+Proof
+  EVAL_TAC >> simp[arr_init_def]
+QED
+
+Theorem arr_init_index_2:
+  array_index arr_init 2 = SOME (IntV (Signed 128) 12)
+Proof
+  EVAL_TAC >> simp[arr_init_def]
+QED
+
+Theorem arr_init_mutable:
+  array_is_mutable arr_init
+Proof
+  simp[arr_init_def]
+QED
+
+Theorem arr_init_length:
+  array_length arr_init = 3
+Proof
+  simp[arr_init_def, array_length_def]
+QED
+
+Theorem arr_init_valid_index:
+  ∀i. valid_index arr_init i ⇔ 0 ≤ i ∧ i < 3
+Proof
+  simp[arr_init_def, array_length_def]
+QED
+
+(* For any valid index of arr_init, the element is a Signed 128 value between 10 and 12 *)
+Theorem arr_init_index_bounds:
+  ∀i. valid_index arr_init i ⇒
+    ∃a. array_index arr_init i = SOME (IntV (Signed 128) a) ∧ 10 ≤ a ∧ a ≤ 12
+Proof
+  rpt strip_tac >>
+  gvs[arr_init_valid_index] >>
+  `i = 0 ∨ i = 1 ∨ i = 2` by ARITH_TAC >>
+  gvs[arr_init_index_0, arr_init_index_1, arr_init_index_2]
 QED
